finished the sample

Test/og/DeviceCacheSimplified.bpl
@@ -1,42 +1,40 @@
-function {:inline} Inv1(currsize: int, newsize: int) : (bool)
+function {:inline} Inv(ghostLock: X, currsize: int, newsize: int) : (bool)
 {
-    currsize <= newsize
+    currsize <= newsize && (ghostLock == nil <==> currsize == newsize)
 }
 
-function {:inline} Inv2(ghostLock: X, currsize: int, newsize: int) : (bool)
-{
-    ghostLock == nil <==> currsize == newsize
-}
-
-procedure Yield({:linear "tid"} tid': X) returns ({:linear "tid"} tid: X)
+procedure YieldToReadCache({:linear "tid"} tid': X) returns ({:linear "tid"} tid: X)
 requires tid' != nil;
+requires Inv(ghostLock, currsize, newsize);
+ensures Inv(ghostLock, currsize, newsize);
+ensures old(currsize) <= currsize;
 ensures tid == tid';
-requires Inv1(currsize, newsize);
-requires Inv2(ghostLock, currsize, newsize);
-ensures Inv1(currsize, newsize);
-ensures Inv2(ghostLock, currsize, newsize);
 {
     assume tid == tid';
-    assert {:yield} Inv1(currsize, newsize);
-    assert Inv2(ghostLock, currsize, newsize);
+    assert {:yield} Inv(ghostLock, currsize, newsize);
+    assert old(currsize) <= currsize;
     assert tid != nil;
 }
 
-procedure YieldWithGhostLock({:linear "tid"} tid': X) returns ({:linear "tid"} tid: X)
+procedure YieldToUpdateCache({:linear "tid"} tid': X, i: int) returns ({:linear "tid"} tid: X)
 requires tid' != nil;
-ensures tid == tid';
-requires Inv1(currsize, newsize);
-requires Inv2(ghostLock, currsize, newsize);
+requires Inv(ghostLock, currsize, newsize);
 requires ghostLock == tid';
-ensures Inv1(currsize, newsize);
-ensures Inv2(ghostLock, currsize, newsize);
+requires currsize <= i;
+ensures Inv(ghostLock, currsize, newsize);
+ensures old(currsize) <= currsize;
+ensures tid == tid';
 ensures ghostLock == tid;
+ensures currsize <= i;
+ensures newsize == old(newsize);
 {
     assume tid == tid';
-    assert {:yield} Inv1(currsize, newsize);
-    assert Inv2(ghostLock, currsize, newsize);
+    assert {:yield} Inv(ghostLock, currsize, newsize);
+    assert old(currsize) <= currsize;
     assert tid != nil;
     assert ghostLock == tid;
+    assert currsize <= i;
+    assert newsize == old(newsize);
 }
 
 var ghostLock: X;
@@ -57,11 +55,10 @@ ensures lock == nil;
 procedure Read ({:linear "tid"} tid': X, start : int, size : int) returns (bytesread : int)
 requires tid' != nil;
 requires 0 <= start && 0 <= size;
-requires Inv1(currsize, newsize);
-requires Inv2(ghostLock, currsize, newsize);
+requires Inv(ghostLock, currsize, newsize);
 ensures 0 <= bytesread && bytesread <= size;
 {
-    var copyGhostLock: X;
+    var copy_currsize: int;
     var i, j, tmp : int;
     var {:linear "tid"} tid: X;
     assume tid == tid';
@@ -71,30 +68,31 @@ ensures 0 <= bytesread && bytesread <= size;
     i := currsize;
     if (start + size <= i) {
         call release(tid); 
-	call tid := Yield(tid);
+	call tid := YieldToReadCache(tid);
 	goto COPY_TO_BUFFER;
     } else if (newsize > i) {
         bytesread := if (start <= i) then (i - start) else 0;
 	call release(tid); 
-	call tid := Yield(tid);
+	call tid := YieldToReadCache(tid);
 	goto COPY_TO_BUFFER;
     } else {
         newsize := start + size;
 	ghostLock := tid;
 	call release(tid); 
-	call tid := YieldWithGhostLock(tid);
+	call tid := YieldToUpdateCache(tid, i);
 	goto READ_DEVICE;
     }
 
 READ_DEVICE:
     while (i < start + size) 
-    invariant Inv1(currsize, newsize);
-    invariant Inv2(ghostLock, currsize, newsize); 
+    invariant Inv(ghostLock, currsize, newsize); 
     invariant ghostLock == tid;
     invariant tid != nil;
+    invariant currsize <= i;
+    invariant newsize == start + size;
     {
-        assert ghostLock == tid;
-        call tid := YieldWithGhostLock(tid);
+        call tid := YieldToUpdateCache(tid, i);
+	assert currsize <= i;
 	i := i + 1;
     }
     call acquire(tid);
@@ -102,24 +100,25 @@ READ_DEVICE:
     currsize := tmp;
     ghostLock := nil;
     call release(tid);
-    call tid := Yield(tid);
+    call tid := YieldToReadCache(tid);
 
 COPY_TO_BUFFER:
     j := 0;
     while(j < bytesread) 
-    invariant Inv1(currsize, newsize);
-    invariant Inv2(ghostLock, currsize, newsize); 
+    invariant 0 <= j;
+    invariant Inv(ghostLock, currsize, newsize); 
     invariant tid != nil;
+    invariant bytesread == 0 || start + bytesread <= currsize;
     {
-        call tid := Yield(tid);
+        call tid := YieldToReadCache(tid);
+	assert start + j < currsize;
         j := j + 1;
     }
 }
 
 procedure thread({:linear "tid"} tid': X)
 requires tid' != nil;
-requires Inv1(currsize, newsize);
-requires Inv2(ghostLock, currsize, newsize);
+requires Inv(ghostLock, currsize, newsize);
 {
     var start, size, bytesread: int;
     var {:linear "tid"} tid: X;
